

## Bayesian Update

- Given new data, old posterior becomes new prior.
- Say we go through  $n$  examples →  $n$  posteriors

Value w/ highest posterior = Maximum a Posteriori (MAP)

$P(D)$  is again product of likelihoods and priors

$$P(D) = \int P(D|H) P(H) dH \quad \text{often intractable}$$

solution

## Conjugate Priors

convenience

prior, posterior from same distribution

simplified calculations

[no need for computing product of likelihood and prior]

product of likelihood and prior gives same distribution as prior with changed parameters

posterior follows known distribution, integral becomes easy; known normalising constant

↓ why?  
god knows

CONJUGATE DISTRIBUTIONS

Beta posterior	Gamma posterior	Gaussian posterior
Beta * Bernoulli	Gamma * Poisson	Normal * Normal
Beta * Binomial	Gamma * exp.	
Beta * -ve binomial		
Beta * geometric		

## Bayesian Linear Regression

- Frequentist linear regression: entirely on data

$$\hat{\beta} = (X^T X)^{-1} X^T y$$

- Small dataset → overfitting
- ∴ Stochastic approach → Bayesian

↓  
distribution of possible values

### NOTE:

- Fewer datapoints → greater uncertainty → greater variation
- All datapoints → Frequentist ≈ Bayes

why?

likelihoods wash out priors

$$P(H|D) \propto P(D|H) P(H) \\ \propto \left[ \prod_{i=1}^M P(D_i|H) \right] P(H) \\ \text{assuming iid}$$

Extremely efficient for tiny dataset  
Well suited for online learning  
No prior knowledge of dataset needed.

Inference takes time  
Not worth it if large amt of data present

## Bayes' Theorem

$$P(H|D) = \frac{P(D|H) \cdot P(H)}{P(D)}$$

posterior      likelihood      prior      normalising factor

likelihood of data given our hypothesis

likelihood of hypothesis before looking at data

$$P(D) = \sum_i \frac{P(D|H_i) P(H_i)}{\text{if } H_i \text{ is true, would I see this data?}} \quad \left. \begin{array}{l} \text{total probability of seeing data over all hypotheses} \\ \text{is } H_i \text{ true?} \end{array} \right\}$$

posterior  $\propto$  likelihood · prior

## Proof: Posterior is Gaussian for Gaussian Prior

Let prior:

$$\beta \sim N(0, S)$$

likelihood:

$$\epsilon | \beta \sim N(0, \sigma^2 I)$$

$$P(\beta | \epsilon) \propto P(\epsilon | \beta) \cdot P(\beta)$$

$$\log P(\beta | \epsilon) \propto \log P(\epsilon | \beta) + \log P(\beta)$$

$$= \log \prod_{j=1}^m \frac{1}{\sqrt{2\pi}\sigma} e^{-\frac{(y_j - (\beta_0 x_{j0} + \dots + \beta_p x_{jp}))^2}{2\sigma^2}} + \log \prod_{j=1}^m \frac{1}{\sqrt{2\pi} S_j} e^{-\frac{\beta_j^2}{2S_j}}$$

$$= \sum_{j=1}^m -\frac{(y_j - (\beta_0 x_{j0} + \dots + \beta_p x_{jp}))^2}{2\sigma^2}$$

$$+ \sum_{j=1}^m -\frac{\beta_j^2}{2S_j} + \text{const}$$

$$= -\frac{1}{2\sigma^2} \|y - X\beta\|^2 - \frac{1}{2} \beta^T S^{-1} \beta + \text{const}$$

$$\begin{aligned} &= -\frac{1}{2\sigma^2} (y - X\beta)^T (y - X\beta) - \frac{1}{2} \beta^T S^{-1} \beta + \text{const} \\ &= -\frac{1}{2\sigma^2} [y^T y - y^T X\beta - \beta^T X^T y + \beta^T X^T X \beta] - \frac{1}{2} \beta^T S^{-1} \beta + \text{const} \\ &= -\frac{1}{2\sigma^2} [y^T y - 2y^T X\beta + \beta^T X^T X \beta] - \frac{1}{2} \beta^T S^{-1} \beta + \text{const} \\ &= -\frac{1}{2} [\beta^T S^{-1} \beta + \frac{\beta^T X^T X \beta}{\sigma^2} - \frac{2y^T X \beta}{\sigma^2}] + \text{const} \\ &= -\frac{1}{2} [\beta^T (S^{-1} + \frac{X^T X}{\sigma^2}) \beta - \frac{2y^T X \beta}{\sigma^2}] + \text{const} \\ &\text{Substitute } Z^{-1} = S^{-1} + \frac{X^T X}{\sigma^2}, \mu = \frac{y^T X}{\sigma^2} \\ &= -\frac{1}{2} [\beta^T (Z^{-1}) \beta - 2\mu] + \text{const} \\ &= -\frac{1}{2} [\beta^T (Z^{-1}) \beta] - \mu + \text{const} \\ &= -\frac{1}{2} (\beta - \mu)^T Z^{-1} (\beta - \mu) \end{aligned}$$

log density of multivariate Gauss